More fixes

new/golang/defn/interface.v
@@ -1,5 +1,11 @@
+From New.golang.defn Require Export postlang.
 
-Definition is_interface_type `{!GoLocalContext} (t : go.type) : bool :=
+Module go.
+Section defs.
+Context {ext : ffi_syntax}.
+Context {go_lctx : GoLocalContext} {go_gctx : GoGlobalContext} `{!GoSemanticsFunctions}.
+
+Definition is_interface_type (t : go.type) : bool :=
   match (to_underlying t) with
   | go.InterfaceType _ => true
   | _ => false
@@ -28,61 +34,18 @@ Definition type_set_contains {go_ctx : GoLocalContext} t t' : bool :=
   | _ => bool_decide (t = t')
   end.
 
-
-
-
-Inductive is_go_step_pure `{!GoGlobalContext} `{!GoLocalContext} :
-  ∀ (op : go_instruction) (arg : val) (e' : expr), Prop :=
-| angelic_exit_step : is_go_step_pure AngelicExit #() (GoInstruction AngelicExit #())%E
-| equals_step t v1 v2 :
-  is_go_step_pure (GoEquals t) (v1, v2)%V (go_eq_top_level t v1 v2)
-| lt_step t v1 v2 :
-  is_go_step_pure (GoLt t) (v1, v2)%V (go_lt t v1 v2)
-| le_step t v1 v2 :
-  is_go_step_pure (GoLe t) (v1, v2)%V (go_le t v1 v2)
-| gt_step t v1 v2 :
-  is_go_step_pure (GoGt t) (v1, v2)%V (go_lt t v2 v1)
-| ge_step t v1 v2 :
-  is_go_step_pure (GoGe t) (v1, v2)%V (go_le t v2 v1)
-| plus_step t v1 v2 :
-  is_go_step_pure (GoPlus t) (v1, v2)%V (go_plus t v1 v2)
-| sub_step t v1 v2 :
-  is_go_step_pure (GoSub t) (v1, v2)%V (go_sub t v1 v2)
-| mul_step t v1 v2 :
-  is_go_step_pure (GoMul t) (v1, v2)%V (go_mul t v1 v2)
-| div_step t v1 v2 :
-  is_go_step_pure (GoDiv t) (v1, v2)%V (go_div t v1 v2)
-| rem_step t v1 v2 :
-  is_go_step_pure (GoRemainder t) (v1, v2)%V (go_remainder t v1 v2)
-| and_step t v1 v2 :
-  is_go_step_pure (GoAnd t) (v1, v2)%V (go_and t v1 v2)
-| or_step t v1 v2 :
-  is_go_step_pure (GoOr t) (v1, v2)%V (go_or t v1 v2)
-| xor_step t v1 v2 :
-  is_go_step_pure (GoXor t) (v1, v2)%V (go_xor t v1 v2)
-| bitclear_step t v1 v2 :
-  is_go_step_pure (GoBitClear t) (v1, v2)%V (go_bitclear t v1 v2)
-| shiftl_step t v1 v2 :
-  is_go_step_pure (GoShiftl t) (v1, v2)%V (go_shiftl t v1 v2)
-| shiftr_step t v1 v2 :
-  is_go_step_pure (GoShiftr t) (v1, v2)%V (go_shiftr t v1 v2)
-
-| load_step t arg : is_go_step_pure (GoLoad t) arg (load t arg)
-| store_step t (l : loc) v : is_go_step_pure (GoStore t) (#l, v)%V (store t #l v)
-| alloc_step t : is_go_step_pure (GoAlloc t) #() (alloc t #())%E
-| prealloc_step (l : loc) : is_go_step_pure GoPrealloc #() #l
-| func_resolve_step f targs : is_go_step_pure (FuncResolve f targs) #() #(functions f targs)
-| method_resolve_step t m : is_go_step_pure (MethodResolve t m) #() #(methods t m)
-| interface_make_step dt v :
-  is_go_step_pure (InterfaceMake dt) v #(interface.mk dt v)
-| interface_get_step m i :
-  is_go_step_pure (InterfaceGet m) #i
+Class InterfaceSemantics :=
+{
+  #[global] interface_make_step dt v ::
+    go.IsGoStepPureDet (InterfaceMake dt) v #(interface.mk dt v);
+  #[global] interface_get_step m i ::
+    go.IsGoStepPureDet (InterfaceGet m) #i
     (match i with
      | interface.nil => Panic "nil dereference in interface call"
-     | interface.mk t v => (GoInstruction (MethodResolve t m) #() v)%E
-     end)
-| type_assert_step t i :
-  is_go_step_pure (TypeAssert t) #i
+     | interface.mk t v => (λ: "arg1", #(methods t m) v "arg1")%E
+     end);
+  #[global] type_assert_step t i ::
+    go.IsGoStepPureDet (TypeAssert t) #i
     (match i with
      | interface.nil => Panic "type assert failed"
      | interface.mk dt v =>
@@ -90,9 +53,9 @@ Inductive is_go_step_pure `{!GoGlobalContext} `{!GoLocalContext} :
            (if (type_set_contains dt t) then #i else Panic "type assert failed")
          else
            (if decide (t = dt) then v else Panic "type assert failed")
-     end)
-| type_assert2_step t i :
-  is_go_step_pure (TypeAssert2 t) #i
+     end);
+  #[global] type_assert2_step t i ::
+    go.IsGoStepPureDet (TypeAssert2 t) #i
     (match i with
      | interface.nil => (#interface.nil, #false)%V
      | interface.mk dt v =>
@@ -100,167 +63,10 @@ Inductive is_go_step_pure `{!GoGlobalContext} `{!GoLocalContext} :
            (if (type_set_contains dt t) then (#i, #true)%V else (#interface.nil, #false)%V)
          else
            (if decide (t = dt) then (v, #true)%V else (go_zero_val t, #false)%E)
-     end)
-| global_var_addr_step v : is_go_step_pure (GlobalVarAddr v) #() #(global_addr v)
-| struct_field_ref_step t f l : is_go_step_pure (StructFieldRef t f) #l #(struct_field_ref t f l)
-| struct_field_get_step t f v :
-  is_go_step_pure (StructFieldGet t f) v (struct_field_get t f v)
-| struct_field_set_step t f v vf :
-  is_go_step_pure (StructFieldSet t f) (v, vf) (struct_field_set t f v vf)
-
-| internal_len_slice_step_pure elem_type s :
-  is_go_step_pure (InternalLen (go.SliceType elem_type)) #s #(s.(slice.len))
-| internal_len_array_step_pure elem_type n v :
-  is_go_step_pure (InternalLen (go.ArrayType n elem_type)) v #(W64 n)
-
-| internal_cap_slice_step_pure elem_type s :
-  is_go_step_pure (InternalCap (go.SliceType elem_type)) #s #(s.(slice.cap))
-| internal_dynamic_array_alloc_pure elem_type (n : w64) :
-  is_go_step_pure (InternalDynamicArrayAlloc elem_type) #n
-    (GoInstruction (GoAlloc $ go.ArrayType (sint.Z n) elem_type) #())
-| internal_slice_make_pure p l c :
-  is_go_step_pure InternalMakeSlice (#p, #l, #c) #(slice.mk p l c)
-| slice_array_step_pure n elem_type p low high:
-  is_go_step_pure (Slice (go.ArrayType n elem_type))
-    (#p, (#low, #high))%V
-    (if decide (0 ≤ sint.Z low ≤ sint.Z high ≤ n) then
-       #(slice.mk (array_index_ref elem_type (sint.Z low) p)
-           (word.sub high low) (word.sub (W64 n) low))
-     else Panic "slice bounds out of range")
-| full_slice_array_step_pure n elem_type p low high max :
-  is_go_step_pure (FullSlice (go.ArrayType n elem_type))
-    (#p, (#low, #high, #max))%V
-    (if decide (0 ≤ sint.Z low ≤ sint.Z high ≤ sint.Z max ∧ sint.Z max ≤ n) then
-       #(slice.mk (array_index_ref elem_type (sint.Z low) p)
-           (word.sub high low) (word.sub max low))
-     else Panic "slice bounds out of range")
-| slice_slice_step_pure elem_type s low high :
-  is_go_step_pure (Slice (go.SliceType elem_type))
-    (#s, (#low, #high))%V
-    (if decide (0 ≤ sint.Z low ≤ sint.Z high ≤ sint.Z s.(slice.cap)) then
-       #(slice.mk (array_index_ref elem_type (sint.Z low) s.(slice.ptr))
-           (word.sub high low) (word.sub s.(slice.cap) low))
-     else Panic "slice bounds out of range")
-| full_slice_slice_step_pure elem_type s low high max :
-  is_go_step_pure (FullSlice (go.SliceType elem_type))
-    (#s, (#low, #high, #max))%V
-    (if decide (0 ≤ sint.Z low ≤ sint.Z high ≤ sint.Z max ∧ sint.Z max ≤ sint.Z s.(slice.cap)) then
-       #(slice.mk (array_index_ref elem_type (sint.Z low) s.(slice.ptr))
-           (word.sub high low) (word.sub max low))
-     else Panic "slice bounds out of range")
-| index_ref_step t v (j : w64) : is_go_step_pure (IndexRef t) (v, #j) (index_ref t (sint.Z j) v)
-| index_step t v (j : w64) : is_go_step_pure (Index t) (v, #j) (index t (sint.Z j) v)
-| array_set_step_pure ty V n (l : array.t ty V n) (v : V) (i : w64) :
-  is_go_step_pure ArraySet (#l, (#i, #v))%V #(array.mk ty n (<[sint.nat i := v ]> (array.arr l)))
-| array_length_step_pure l :
-  is_go_step_pure ArrayLength (ArrayV l)
-    (if decide (length l < 2^63) then
-       #(W64 (length l))
-     else (GoInstruction AngelicExit #()))
-| internal_map_lookup_step_pure m k :
-  is_go_step_pure InternalMapLookup (m, k) (let '(ok, v) := map_lookup m k in (v, #ok))
-| internal_map_insert_step_pure m k v :
-  is_go_step_pure InternalMapInsert (m, k, v) (map_insert m k v)
-| internal_map_delete_step_pure m k :
-  is_go_step_pure InternalMapDelete (m, k) (map_delete m k)
-| internal_map_length_step_pure m ks (H : is_map_domain m ks) :
-  is_go_step_pure InternalMapLength m #(W64 (length ks))
-| internal_map_domain_literal_step_pure m ks (H : is_map_domain m ks) :
-  is_go_step_pure InternalMapDomainLiteral m
-    (LiteralValue ((λ v, KeyedElement None $ ElementExpression $ Val v) <$> ks))
-| internal_map_make_step_pure v :
-  is_go_step_pure InternalMapMake v (map_empty v)
-| composite_literal_step t v :
-  is_go_step_pure (CompositeLiteral t) v (composite_literal t v)
-.
-
+     end);
 
   method_interface t m (H : is_interface_type t = true) :
     #(methods t m) = (InterfaceGet m);
-
-
-
-
-    go_eq_top_level := inhabitant;
-    go_lt := inhabitant;
-    go_le := inhabitant;
-    go_plus := inhabitant;
-    go_sub := inhabitant;
-    go_mul := inhabitant;
-    go_div := inhabitant;
-    go_remainder := inhabitant;
-    go_and := inhabitant;
-    go_or := inhabitant;
-    go_xor := inhabitant;
-    go_bitclear := inhabitant;
-    go_shiftl := inhabitant;
-    go_shiftr := inhabitant;
-    global_addr := inhabitant;
-    functions := inhabitant;
-    methods := inhabitant;
-    method_set := inhabitant;
-    alloc := inhabitant;
-    load := inhabitant;
-    store := inhabitant;
-    go_zero_val := inhabitant;
-    struct_field_ref := inhabitant;
-    struct_field_get := inhabitant;
-    struct_field_set := inhabitant;
-    index := inhabitant;
-    index_ref := inhabitant;
-    array_index_ref := inhabitant;
-    to_underlying := inhabitant;
-    map_empty := inhabitant;
-    map_lookup := inhabitant;
-    map_insert := inhabitant;
-    map_delete := inhabitant;
-    is_map_domain := inhabitant;
-    composite_literal := inhabitant;
-  |}.
-
-
-Global Instance pure_wp_TypeAssert_non_interface t v :
-  PureWp (is_interface_type t = false) (TypeAssert t #(interface.mk t v)) v.
-Proof.
-  iIntros "% * %Heq % HΦ"; iApply wp_GoInstruction; [ intros; repeat econstructor |  ]; iNext.
-  iIntros "* %Hstep Hlc". inv Hstep. inv Hpure. iIntros "$ !>".
-  simpl. rewrite Heq. rewrite decide_True //. by iApply "HΦ".
-Qed.
-
-Global Instance pure_wp_TypeAssert_interface t dt v :
-  PureWp (is_interface_type t = true ∧ type_set_contains dt t = true)
-    (TypeAssert t #(interface.mk dt v)) #(interface.mk dt v).
-Proof.
-  iIntros "% * %Heq % HΦ"; iApply wp_GoInstruction; [ intros; repeat econstructor |  ]; iNext.
-  iIntros "* %Hstep Hlc". inv Hstep. inv Hpure. iIntros "$ !>".
-  simpl. destruct Heq as [-> Hcontains]. rewrite Hcontains. by iApply "HΦ".
-Qed.
-
-Global Instance pure_wp_TypeAssert2_non_interface t t' `{!ZeroVal V}
-                `{!go.GoZeroValEq t V} `{!TypedPointsto V} `{!IntoValTyped V t} (v : V) :
-  PureWp (is_interface_type t = false)
-    (TypeAssert2 t #(interface.mk t' #v))
-    (if decide (t = t') then (#v, #true)%V else (#(zero_val V), #false)%V).
-Proof.
-  iIntros "% * %Heq % HΦ"; iApply wp_GoInstruction; [ intros; repeat econstructor |  ]; iNext.
-  iIntros "* %Hstep Hlc". inv Hstep. inv Hpure. iIntros "$ !>".
-  simpl. rewrite Heq. destruct decide.
-  - by iApply "HΦ".
-  - rewrite go.go_zero_val_eq. wp_pures. by iApply "HΦ".
-Qed.
-
-Global Instance pure_wp_TypeAssert2_interface t i :
-  PureWp (is_interface_type t = true)
-    (TypeAssert2 t #i)
-    (match i with
-     | interface.mk dt v =>
-         if type_set_contains dt t then (# i, # true)%V else (# interface.nil, # false)%V
-     | interface.nil => (# interface.nil, # false)%V
-     end).
-Proof.
-  iIntros "% * %Heq % HΦ"; iApply wp_GoInstruction; [ intros; repeat econstructor |  ]; iNext.
-  iIntros "* %Hstep Hlc". inv Hstep. inv Hpure. iIntros "$ !>".
-  simpl. rewrite Heq. destruct i.
-  - by iApply "HΦ".
-  - by iApply "HΦ".
-Qed.
+}.
+End defs.
+End go.
