new/golang/theory/auto.v
@@ -1,9 +1,8 @@
-From Perennial.goose_lang Require Import notation.
 From Coq Require Import ssreflect.
 From Ltac2 Require Import Ltac2 Printf.
 Set Default Proof Mode "Classic".
-From New.golang.theory Require Import proofmode pkg loop.
-From New.golang.theory Require Import mem.
+From New.golang.theory Require Export proofmode pkg loop.
+From New.golang.theory Require Export mem.
 From Perennial Require Import base.
 
 #[local] Open Scope general_if_scope.
@@ -339,113 +338,3 @@ Ltac wp_end :=
       iFrame;
       word
   ].
-
-Section __struct_test.
-Context `{sem: ffi_semantics} `{!ffi_interp ffi} `{!heapGS Σ}
-  {core_sem : go.CoreSemantics} {pre_sem : go.PredeclaredSemantics}.
-
-Record foo_t :=
-  mk {
-      a : w64;
-      b : go_string;
-    }.
-Global Instance settable_foo : Settable foo_t :=
-  settable! mk < a; b >.
-
-Definition foo_impl : go.type := go.StructType [(go.FieldDecl "a"%go go.uint64); (go.EmbeddedField "b"%go go.string)].
-Definition foo : go.type := go.Named "foo"%go [].
-Axiom zero_val_foo : ZeroVal foo_t.
-Global Existing Instance zero_val_foo.
-
-Class foo_type_assumptions : Prop :=
-  {
-    foo_underlying : to_underlying foo = foo_impl;
-    foo_zero_val : zero_val foo_t = mk (zero_val _) (zero_val _);
-    foo_go_zero_val : go_zero_val foo = #(zero_val foo_t);
-    foo_impl_go_zero_val : go_zero_val foo_impl = #(zero_val foo_t);
-    #[global] foo_get_a x :: go.IsGoStepPureDet (StructFieldGet foo "a") #x #x.(a);
-    #[global] foo_get_b x :: go.IsGoStepPureDet (StructFieldGet foo "b") #x #x.(b);
-    #[global] foo_set_a x a' :: go.IsGoStepPureDet (StructFieldSet foo "a") (#x, #a')%V #(x <|a := a'|>);
-    #[global] foo_set_b x b' :: go.IsGoStepPureDet (StructFieldSet foo "b") (#x, #b')%V #(x <|b := b'|>);
-    #[global] foo_impl_get_a x :: go.IsGoStepPureDet (StructFieldGet foo_impl "a") #x #x.(a);
-    #[global] foo_impl_get_b x :: go.IsGoStepPureDet (StructFieldGet foo_impl "b") #x #x.(b);
-    #[global] foo_impl_set_a x a' :: go.IsGoStepPureDet (StructFieldSet foo_impl "a") (#x, #a') #(x <|a := a'|>);
-    #[global] foo_impl_set_b x b' :: go.IsGoStepPureDet (StructFieldSet foo_impl "b") (#x, #b') #(x <|b := b'|>);
-  }.
-
-Program Global Instance typed_pointsto_foo : TypedPointsto foo_t :=
-  {| typed_pointsto_def l dq v :=
-      ("a" ∷ struct_field_ref foo "a"%go l ↦{dq} v.(a) ∗
-       "b" ∷ struct_field_ref foo "b"%go l ↦{dq} v.(b)
-      )%I |}.
-Final Obligation.
-Proof.
-simpl. intros. iNamedSuffix 1 "1". iNamedSuffix 1 "2".
-destruct v1, v2; simpl.
-iCombine "a1 a2" gives %->.
-iCombine "b1 b2" gives %->.
-done.
-Qed.
-
-Context `{!foo_type_assumptions}.
-
-Global Instance into_val_typed_foo  : IntoValTyped foo_t foo.
-Proof using H core_sem pre_sem.
-  split.
-  - iIntros "* _ HΦ".
-    rewrite go.alloc_underlying foo_underlying.
-    rewrite go.alloc_struct.
-    rewrite [in (_ (foo_t))]typed_pointsto_unseal /=.
-    rewrite go.struct_field_ref_underlying foo_underlying.
-    wp_auto.
-    wp_apply wp_GoPrealloc. iIntros (l) "_".
-
-    wp_auto.
-    case_bool_decide; subst; wp_pures; last (wp_apply wp_AngelicExit).
-    iDestruct "l_field" as "?".
-
-    wp_auto. case_bool_decide; subst; wp_pures; last (wp_apply wp_AngelicExit).
-
-    iApply "HΦ". rewrite foo_zero_val. iFrame.
-  - iIntros "* Hl HΦ".
-    rewrite [in (_ (foo_t))]typed_pointsto_unseal /=.
-    rewrite go.load_underlying foo_underlying.
-    rewrite go.struct_field_ref_underlying foo_underlying.
-    rewrite go.load_struct /=.
-    iNamed "Hl".
-
-    wp_pures. wp_apply (wp_load with "[$a]"). iIntros "a". wp_pures.
-
-    wp_bind. rewrite foo_impl_go_zero_val.
-    wp_pures. wp_apply (wp_load with "[$b]"). iIntros "b". wp_pures.
-
-    destruct v. iApply "HΦ". iFrame.
-  - iIntros "* Hl HΦ".
-    rewrite [in (_ (foo_t))]typed_pointsto_unseal /=.
-    rewrite go.store_underlying foo_underlying.
-    rewrite go.struct_field_ref_underlying foo_underlying.
-    rewrite go.store_struct /=. iNamed "Hl".
-
-    wp_pures. wp_apply (wp_store with "a"). iIntros "a".
-    wp_pures. wp_apply (wp_store with "b"). iIntros "b".
-
-    iApply "HΦ". iFrame.
-Qed.
-
-Lemma wp_test :
-  {{{ True }}}
-    (let: "i" := #(interface.mk (go.uint64) #(W64 0)) in
-     let: "z" := MethodResolve (go.error) "foo" #() "i" in
-     #()
-    )
-  {{{ RET #(); True }}}.
-Proof.
-  iIntros "% _ HΦ". wp_pures.
-  rewrite go.method_interface //.
-  2:{ unfold is_interface_type. erewrite go.predeclared_underlying.
-      2:{ admit. }
-      done. }
-  wp_auto.
-Abort.
-
-End __struct_test.
