new/golang/theory/test.v
@@ -1,38 +1,109 @@
-From New.golang.theory Require Export postlifting.
+From New.golang.theory Require Export auto.
 
 Section test.
-Context `{sem: ffi_semantics} `{!ffi_interp ffi} `{!heapGS Σ} {core_sem : go.CoreSemantics}.
+Context `{sem: ffi_semantics} `{!ffi_interp ffi} `{!heapGS Σ}
+  {core_sem : go.CoreSemantics} {pre_sem : go.PredeclaredSemantics}
+  {interface_sem : go.InterfaceSemantics}.
 
-Definition someStructType : go.type :=
-  go.StructType [(go.FieldDecl "a"%go (go.PointerType (go.Named "uint64"%go [])))].
+Record foo_t :=
+  mk {
+      a : w64;
+      b : go_string;
+    }.
+Global Instance settable_foo : Settable foo_t :=
+  settable! mk < a; b >.
 
-Lemma wp_test  :
-  {{{ True }}}
-  GoEquals someStructType (StructV {[ "a"%go := #null ]}, StructV {[ "a"%go := #null ]})%V
-  {{{ RET #true; True }}}.
+Definition foo_impl : go.type := go.StructType [(go.FieldDecl "a"%go go.uint64); (go.EmbeddedField "b"%go go.string)].
+Definition foo : go.type := go.Named "foo"%go [].
+Axiom zero_val_foo : ZeroVal foo_t.
+Global Existing Instance zero_val_foo.
+
+Class foo_type_assumptions : Prop :=
+  {
+    foo_underlying : to_underlying foo = foo_impl;
+    foo_zero_val : zero_val foo_t = mk (zero_val _) (zero_val _);
+    foo_go_zero_val : go_zero_val foo = #(zero_val foo_t);
+    foo_impl_go_zero_val : go_zero_val foo_impl = #(zero_val foo_t);
+    #[global] foo_get_a x :: go.IsGoStepPureDet (StructFieldGet foo "a") #x #x.(a);
+    #[global] foo_get_b x :: go.IsGoStepPureDet (StructFieldGet foo "b") #x #x.(b);
+    #[global] foo_set_a x a' :: go.IsGoStepPureDet (StructFieldSet foo "a") (#x, #a')%V #(x <|a := a'|>);
+    #[global] foo_set_b x b' :: go.IsGoStepPureDet (StructFieldSet foo "b") (#x, #b')%V #(x <|b := b'|>);
+    #[global] foo_impl_get_a x :: go.IsGoStepPureDet (StructFieldGet foo_impl "a") #x #x.(a);
+    #[global] foo_impl_get_b x :: go.IsGoStepPureDet (StructFieldGet foo_impl "b") #x #x.(b);
+    #[global] foo_impl_set_a x a' :: go.IsGoStepPureDet (StructFieldSet foo_impl "a") (#x, #a') #(x <|a := a'|>);
+    #[global] foo_impl_set_b x b' :: go.IsGoStepPureDet (StructFieldSet foo_impl "b") (#x, #b') #(x <|b := b'|>);
+  }.
+
+Program Global Instance typed_pointsto_foo : TypedPointsto foo_t :=
+  {| typed_pointsto_def l dq v :=
+      ("a" ∷ struct_field_ref foo "a"%go l ↦{dq} v.(a) ∗
+       "b" ∷ struct_field_ref foo "b"%go l ↦{dq} v.(b)
+      )%I |}.
+Final Obligation.
 Proof.
-  iIntros "% _ HΦ".
+simpl. intros. iNamedSuffix 1 "1". iNamedSuffix 1 "2".
+destruct v1, v2; simpl.
+iCombine "a1 a2" gives %->.
+iCombine "b1 b2" gives %->.
+done.
+Qed.
 
-  (* TODO: abstract into lemma *)
-  iApply (wp_GoInstruction [] (GoEquals someStructType)).
-  { intros. repeat econstructor. }
-  iNext; iIntros "* %Hstep"; inv Hstep; inv Hpure.
-  iIntros "? $ !>". simpl.
+Context `{!foo_type_assumptions}.
 
-  (* precondition/typeclass *)
-  assert (go.is_comparable someStructType) as Hcomp.
-  { rewrite go.is_comparable_struct. repeat constructor. apply into_val_comparable. }
-  rewrite Hcomp.
+Global Instance into_val_typed_foo  : IntoValTyped foo_t foo.
+Proof using H core_sem pre_sem.
+  split.
+  - iIntros "* _ HΦ".
+    rewrite go.alloc_underlying foo_underlying.
+    rewrite go.alloc_struct.
+    rewrite [in (_ (foo_t))]typed_pointsto_unseal /=.
+    rewrite go.struct_field_ref_underlying foo_underlying.
+    wp_auto.
+    wp_apply wp_GoPrealloc. iIntros (l) "_".
 
-  rewrite go._go_eq_struct. simpl.
-  wp_pures.
-  wp_apply wp_StructFieldGet_untyped. (* TODO: use struct field get instance *)
-  { rewrite lookup_singleton //. }
-  iIntros "_".
-  wp_apply wp_StructFieldGet_untyped.
-  { rewrite lookup_singleton //. }
-  iIntros "_".
-  wp_pures. by iApply "HΦ".
+    wp_auto.
+    case_bool_decide; subst; wp_pures; last (wp_apply wp_AngelicExit).
+    iDestruct "l_field" as "?".
+
+    wp_auto. case_bool_decide; subst; wp_pures; last (wp_apply wp_AngelicExit).
+
+    iApply "HΦ". rewrite foo_zero_val. iFrame.
+  - iIntros "* Hl HΦ".
+    rewrite [in (_ (foo_t))]typed_pointsto_unseal /=.
+    rewrite go.load_underlying foo_underlying.
+    rewrite go.struct_field_ref_underlying foo_underlying.
+    rewrite go.load_struct /=.
+    iNamed "Hl".
+
+    wp_pures. wp_apply (wp_load with "[$a]"). iIntros "a". wp_pures.
+
+    wp_bind. rewrite foo_impl_go_zero_val.
+    wp_pures. wp_apply (wp_load with "[$b]"). iIntros "b". wp_pures.
+
+    destruct v. iApply "HΦ". iFrame.
+  - iIntros "* Hl HΦ".
+    rewrite [in (_ (foo_t))]typed_pointsto_unseal /=.
+    rewrite go.store_underlying foo_underlying.
+    rewrite go.struct_field_ref_underlying foo_underlying.
+    rewrite go.store_struct /=. iNamed "Hl".
+
+    wp_pures. wp_apply (wp_store with "a"). iIntros "a".
+    wp_pures. wp_apply (wp_store with "b"). iIntros "b".
+
+    iApply "HΦ". iFrame.
+Qed.
+
+Lemma wp_test T V (v : V) :
+  {{{ {{{ True }}} #(methods T "Error") #v #() {{{ (s : go_string), RET #s; True }}} }}}
+    (let: "i" := #(interface.mk T #v) in
+     let: "z" := MethodResolve (go.error) "Error" #() "i" in
+     "z" #())
+  {{{ (s : go_string), RET #s; True }}}.
+Proof.
+  iIntros "% #He HΦ". wp_pures.
+  rewrite (go.method_interface go.error).
+  2:{ rewrite /go.is_interface_type go.to_underlying_not_named //. }
+  wp_auto. wp_apply "He" as "% _". by iApply "HΦ".
 Qed.
 
 End test.
