new/golang/defn/map.v
@@ -65,6 +65,20 @@ Context {ext : ffi_syntax}.
 Context {go_lctx : GoLocalContext} {go_gctx : GoGlobalContext}.
 Class MapSemantics `{!GoSemanticsFunctions} :=
 {
+  #[global] internal_map_lookup_step_pure m k ::
+    go.IsGoStepPureDet InternalMapLookup (m, k) (let '(ok, v) := map_lookup m k in (v, #ok));
+  #[global] internal_map_insert_step_pure m k v ::
+    go.IsGoStepPureDet InternalMapInsert (m, k, v) (map_insert m k v);
+  #[global] internal_map_delete_step_pure m k ::
+    go.IsGoStepPureDet InternalMapDelete (m, k) (map_delete m k);
+  #[global] internal_map_length_step_pure m ks (H : is_map_domain m ks) ::
+    go.IsGoStepPureDet InternalMapLength m #(W64 (length ks));
+  #[global] internal_map_domain_literal_step_pure m ks (H : is_map_domain m ks) ::
+    go.IsGoStepPureDet InternalMapDomainLiteral m
+    (LiteralValue ((λ v, KeyedElement None $ ElementExpression $ Val v) <$> ks));
+  #[global] internal_map_make_step_pure v ::
+    go.IsGoStepPureDet InternalMapMake v (map_empty v);
+
   (* special cases for equality *)
   #[global] is_go_op_go_equals_map_nil_l kt vt s ::
     go.IsGoOp GoEquals (go.MapType kt vt) (#map.nil, #s)%V #(bool_decide (s = map.nil));
